<?xml version="1.0"?>
<rdf:RDF xmlns="http://purl.obolibrary.org/obo/litero.owl#"
     xml:base="http://purl.obolibrary.org/obo/litero.owl"
     xmlns:dc="http://purl.org/dc/elements/1.1/"
     xmlns:obo="http://purl.obolibrary.org/obo/"
     xmlns:owl="http://www.w3.org/2002/07/owl#"
     xmlns:rdf="http://www.w3.org/1999/02/22-rdf-syntax-ns#"
     xmlns:xml="http://www.w3.org/XML/1998/namespace"
     xmlns:xsd="http://www.w3.org/2001/XMLSchema#"
     xmlns:foaf="http://xmlns.com/foaf/0.1/"
     xmlns:rdfs="http://www.w3.org/2000/01/rdf-schema#"
     xmlns:terms="http://purl.org/dc/terms/"
     xmlns:protege="http://protege.stanford.edu/plugins/owl/protege#"
     xmlns:oboInOwl="http://www.geneontology.org/formats/oboInOwl#"
     xmlns:ace_lexicon="http://attempto.ifi.uzh.ch/ace_lexicon#">
    <owl:Ontology rdf:about="http://purl.obolibrary.org/obo/litero.owl">
        <owl:imports rdf:resource="http://purl.obolibrary.org/obo/MF/2020-08-07/MF.owl"/>
        <owl:imports rdf:resource="http://purl.obolibrary.org/obo/MFOEM/2020-05-13/MFOEM.owl"/>
        <owl:imports rdf:resource="http://purl.obolibrary.org/obo/bfo/2019-08-26/bfo.owl"/>
        <owl:imports rdf:resource="http://purl.obolibrary.org/obo/iao/2020-06-10/iao.owl"/>
        <rdfs:comment>Literature Ontology: an ontology for literary works and associated entities.</rdfs:comment>
    </owl:Ontology>
    


    <!-- 
    ///////////////////////////////////////////////////////////////////////////////////////
    //
    // Classes
    //
    ///////////////////////////////////////////////////////////////////////////////////////
     -->

    


    <!-- http://purl.obolibrary.org/obo/LITERO_000015 -->

    <owl:Class rdf:about="http://purl.obolibrary.org/obo/LITERO_000015">
        <rdfs:subClassOf rdf:resource="http://purl.obolibrary.org/obo/LITERO_000019"/>
        <obo:IAO_0000115>A fictional work that is the length of a book.</obo:IAO_0000115>
        <rdfs:label xml:lang="en">novel</rdfs:label>
    </owl:Class>
    


    <!-- http://purl.obolibrary.org/obo/LITERO_000016 -->

    <owl:Class rdf:about="http://purl.obolibrary.org/obo/LITERO_000016">
        <rdfs:subClassOf rdf:resource="http://purl.obolibrary.org/obo/BFO_0000031"/>
        <obo:IAO_0000115>A generically dependent continuant that consists of a written work that has aesthetic value and artistic merit.</obo:IAO_0000115>
        <rdfs:label xml:lang="en">literary work</rdfs:label>
    </owl:Class>
    


    <!-- http://purl.obolibrary.org/obo/LITERO_000017 -->

    <owl:Class rdf:about="http://purl.obolibrary.org/obo/LITERO_000017">
        <rdfs:subClassOf rdf:resource="http://purl.obolibrary.org/obo/LITERO_000016"/>
        <obo:IAO_0000115>A literary work in which the expression of feelings and ideas is given through style and the interplay of words and rhythm.</obo:IAO_0000115>
        <obo:comment>Poetry often employs rhyme and meter.</obo:comment>
        <rdfs:label xml:lang="en">poetry</rdfs:label>
    </owl:Class>
    


    <!-- http://purl.obolibrary.org/obo/LITERO_000018 -->

    <owl:Class rdf:about="http://purl.obolibrary.org/obo/LITERO_000018">
        <rdfs:subClassOf rdf:resource="http://purl.obolibrary.org/obo/BFO_0000031"/>
        <obo:IAO_0000115>A generically dependent continuant that is part of a work of fiction and appears to be about some thing.</obo:IAO_0000115>
        <rdfs:label xml:lang="en">fictional content entity</rdfs:label>
    </owl:Class>
    


    <!-- http://purl.obolibrary.org/obo/LITERO_000019 -->

    <owl:Class rdf:about="http://purl.obolibrary.org/obo/LITERO_000019">
        <rdfs:subClassOf rdf:resource="http://purl.obolibrary.org/obo/LITERO_000016"/>
        <obo:IAO_0000115>A literary work that is about people, objects and situations that do not really exist.</obo:IAO_0000115>
        <rdfs:label xml:lang="en">fictional work</rdfs:label>
    </owl:Class>
    


    <!-- http://purl.obolibrary.org/obo/LITERO_000020 -->

    <owl:Class rdf:about="http://purl.obolibrary.org/obo/LITERO_000020">
        <rdfs:subClassOf rdf:resource="http://purl.obolibrary.org/obo/LITERO_000018"/>
        <obo:IAO_0000115>A fictional content entity that appears to be about a person.</obo:IAO_0000115>
        <rdfs:label xml:lang="en">fictional character</rdfs:label>
    </owl:Class>
    


    <!-- 
    ///////////////////////////////////////////////////////////////////////////////////////
    //
    // Individuals
    //
    ///////////////////////////////////////////////////////////////////////////////////////
     -->

    


    <!-- http://purl.obolibrary.org/obo/LITERO_000021 -->

    <owl:NamedIndividual rdf:about="http://purl.obolibrary.org/obo/LITERO_000021">
        <rdf:type rdf:resource="http://purl.obolibrary.org/obo/MF_0000016"/>
        <rdfs:label xml:lang="en">Charlotte Bronte</rdfs:label>
    </owl:NamedIndividual>
</rdf:RDF>



<!-- Generated by the OWL API (version 4.5.9.2019-02-01T07:24:44Z) https://github.com/owlcs/owlapi -->

